fill some admit

Diff/NonRobustDef.v
@@ -27,10 +27,10 @@ Section Preservation.
   Variable S__S : EndState States__S.
   Variable S__T : EndState States__T.
 
-  Local Definition trace__S := trace Σ__S States__S. 
-  Local Definition trace__T := trace Σ__T States__T.  
-  Local Definition prop__S := prop Σ__S States__S.
-  Local Definition prop__T := prop Σ__T States__T.
+  Definition trace__S := trace Σ__S States__S. 
+  Definition trace__T := trace Σ__T States__T.  
+  Definition prop__S := prop Σ__S States__S.
+  Definition prop__T := prop Σ__T States__T.
 
   Variable sem__S : prg Source -> trace__S -> Prop.
   Variable non_empty_sem__S : forall W, exists s, sem__S W s.   
@@ -38,15 +38,15 @@ Section Preservation.
   Variable sem__T : prg Target -> trace__T -> Prop.
   Variable non_empty_sem__T : forall W, exists t, sem__T W t.   
   
-  Local Definition prg__S := prg Source.
-  Local Definition prg__T := prg Target.
+  Definition prg__S := prg Source.
+  Definition prg__T := prg Target.
 
-  Local Definition sat__S := sat Source sem__S.
-  Local Definition sat__T := sat Target sem__T.
+  Definition sat__S := sat Source sem__S.
+  Definition sat__T := sat Target sem__T.
   
-  Local Definition cmp := compile_whole Source Target compilation_chain.
+  Definition cmp := compile_whole Source Target compilation_chain.
 
-  Local Notation "W ↓" := (cmp W) (at level 50).  
+  Notation "W ↓" := (cmp W) (at level 50).  
 
   (* parameters *)
   
@@ -61,30 +61,51 @@ Section Preservation.
 
   Definition σTP := forall W π__T, σP W π__T.
 
+  Lemma contra_σP (W : prg__S) (π__T : prop__T) :
+    (σP W π__T) <->  ((exists t, sem__T (W ↓) t /\ ~ (π__T t)) ->
+                  (exists s, sem__S W s /\ ~ (σ π__T) s)). 
+  Proof.
+    rewrite /σP. by rewrite [_ -> _] contra !neg_sat. 
+  Qed. 
+  
   Lemma contra_σTP :
     σTP <-> (forall W π__T, (exists t, sem__T (W ↓) t /\ ~ (π__T t)) ->
-                    (exists s, sem__S W s /\ ~ (σ π__T) s)).
-  Proof. Admitted. (*TODO: see contra_σRTP in previous files *)
-  
+                   (exists s, sem__S W s /\ ~ (σ π__T) s)).
+  Proof.
+    rewrite /σTP.
+    split => H W π__T; by move/contra_σP: (H W π__T).
+  Qed.
+
   Definition τP (W : prg__S) (π__S : prop__S) :=
     sat__S W π__S -> sat__T (W ↓) (τ π__S).
 
   Definition τTP := forall W π__S, τP W π__S.
 
-   Lemma contra_τTP :
-    τTP <-> (forall W π__S, (exists t, sem__T (W ↓) t /\ ~ (τ π__S) t) ->
-                    (exists s, sem__S W s /\ ~ π__S s)).
-  Proof. Admitted. (*TODO: see contra_τRTP in previous files *)
 
+  Lemma contra_τP (W : prg__S) (π__S : prop__S) :
+    (τP W π__S) <-> ((exists t, sem__T (W ↓) t /\ ~ (τ π__S) t) ->
+                 (exists s, sem__S W s /\ ~ π__S s)).
+  Proof.
+    rewrite /τP. by rewrite [_ -> _] contra !neg_sat. 
+  Qed.      
+  
+  Lemma contra_τTP :
+    τTP <-> (forall W π__S, (exists t, sem__T (W ↓) t /\ ~ (τ π__S) t) ->
+                   (exists s, sem__S W s /\ ~ π__S s)).
+  Proof.
+    rewrite /τTP.
+    split => H W π__S; by move/contra_τP: (H W π__S).
+  Qed.
+  
   Theorem G_σTP_iff_τTP :
     (Galois_fst τ σ) -> (Galois_snd τ σ) -> (σTP <-> τTP).
   Proof.
-     move => G1 G2. split. 
-     - move => Hσ P πs Hsat_src. apply: (Hσ P (τ πs)).
-       apply: sat_upper_closed. exact Hsat_src. by apply: G1. 
-     - move => Hτ P πt Hrsat_tgt.
-       have H : sat__T (P ↓) (τ (σ πt)) by apply: Hτ. 
-       apply: sat_upper_closed. exact H. by apply: G2.
+    move => G1 G2. split. 
+    - move => Hσ P πs Hsat_src. apply: (Hσ P (τ πs)).
+      apply: sat_upper_closed. exact Hsat_src. by apply: G1. 
+    - move => Hτ P πt Hrsat_tgt.
+      have H : sat__T (P ↓) (τ (σ πt)) by apply: Hτ. 
+      apply: sat_upper_closed. exact H. by apply: G2.
   Qed.     
 
   Corollary Adj_σTP_iff_τTP :
@@ -93,8 +114,7 @@ Section Preservation.
     rewrite Galois_equiv. move => [ms [mt [G1 G2]]].
       by apply: G_σTP_iff_τTP. 
   Qed. 
-      
+  
 End Preservation.                                      
-
 
 
